theories/LambdaSepROMosel.v
@@ -334,7 +334,7 @@ Proof. by rewrite /PrepareHProp=>-> ->. Qed.
 
 Lemma rule_ramified_frame_read_only_absorb : forall t H Q H' Q',
   triple t H' Q' ->
-  H ==> (<absorb> ROFrame H' (normally (Q' \---* Q)))%I ->
+  H ==> (<absorb> ROFrame H' (normally (Q' \--* Q)))%I ->
   triple t H Q.
 Proof using.
   intros t H Q H' Q' Ht HH. eapply rule_consequence; first last; [done| |].
@@ -345,7 +345,7 @@ Qed.
 
 Lemma rule_ramified_frame_read_only_absorb_locked : forall t H Q H' Q',
   triple t H' Q' ->
-  H ==> (<absorb> ROFrame H' (normally (locked Q' \---* Q)))%I ->
+  H ==> (<absorb> ROFrame H' (normally (locked Q' \--* Q)))%I ->
   triple t H Q.
 Proof using. unlock. apply rule_ramified_frame_read_only_absorb. Qed.
 
@@ -358,7 +358,7 @@ Ltac ram_apply lem :=
 
 Lemma rule_let_ramified_frame_read_only_locked : forall z t1 t2 H1 H Q1 Q Q',
   triple t1 H1 Q1 ->
-  H ==> ROFrame H1 (locked Q1 \---* Q') ->
+  H ==> ROFrame H1 (locked Q1 \--* Q') ->
   (forall (X:val), triple (subst1 z X t2) (Q' X) Q) ->
   triple (trm_let z t1 t2) H Q.
 Proof using. unlock. apply rule_let_ramified_frame_read_only. Qed.
